the definition of [read] finally type-checks

src/BasicProg.v
@@ -110,16 +110,6 @@ Qed.
 Hint Extern 1 ({{_}} If_ _ _ _ >> _) => apply if_ok : prog.
 Notation "'If' b { p1 } 'else' { p2 }" := (If_ b p1 p2) (at level 9, b at level 0).
 
-Fixpoint For_ (L : Set) (G : Type) (f : nat -> L -> (L -> prog) -> prog)
-              (i n : nat) (l : L)
-              (nocrash : G -> nat -> L -> pred)
-              (crashed : G -> pred)
-              (rx: L -> prog) : prog :=
-  match n with
-    | O => rx l
-    | S n' => l' <- (f i l); (For_ f (S i) n' l' nocrash crashed rx)
-  end.
-
 Record For_args (L : Set) := {
   For_args_i : addr;
   For_args_n : addr;
@@ -135,22 +125,21 @@ Proof.
   apply wlt_lt; auto.
 Qed.
 
-Definition For_loop (L : Set) (G : Type) (f : addr -> L -> (L -> prog) -> prog)
-                    (i n : addr) (l : L)
-                    (nocrash : G -> addr -> L -> pred)
-                    (crashed : G -> pred)
-                    (rx: L -> prog)
-                    : prog.
+Definition For_ (L : Set) (G : Type) (f : addr -> L -> (L -> prog) -> prog)
+                (i n : addr) (l : L)
+                (nocrash : G -> addr -> L -> pred)
+                (crashed : G -> pred)
+                (rx: L -> prog) : prog.
   refine (Fix (@for_args_wf L) (fun _ => prog)
-          (fun args For_loop => _)
+          (fun args For_ => _)
           {| For_args_i := i; For_args_n := n; For_args_l := l |}).
   clear i n l.
   destruct args.
   refine (if weq For_args_n0 (natToWord addrlen 0) then rx For_args_l0 else _).
   refine (l' <- (f For_args_i0 For_args_l0); _).
-  refine (For_loop {| For_args_i := For_args_i0 ^+ (natToWord addrlen 1);
-                      For_args_n := For_args_n0 ^- (natToWord addrlen 1);
-                      For_args_l := l' |} _).
+  refine (For_ {| For_args_i := For_args_i0 ^+ (natToWord addrlen 1);
+                  For_args_n := For_args_n0 ^- (natToWord addrlen 1);
+                  For_args_l := l' |} _).
 
   assert (wordToNat For_args_n0 <> 0).
   unfold not in *; intros; apply n.
@@ -178,18 +167,18 @@ Definition For_loop (L : Set) (G : Type) (f : addr -> L -> (L -> prog) -> prog)
   omega.
 Defined.
 
-Lemma For_loop_step: forall L G f i n l nocrash crashed rx,
-  @For_loop L G f i n l nocrash crashed rx =
+Lemma For_step: forall L G f i n l nocrash crashed rx,
+  @For_ L G f i n l nocrash crashed rx =
     if weq n (natToWord addrlen 0)
     then rx l
     else l' <- (f i l);
-         @For_loop L G f
-                   (i ^+ (natToWord addrlen 1))
-                   (n ^- (natToWord addrlen 1))
-                   l' nocrash crashed rx.
+         @For_ L G f
+               (i ^+ (natToWord addrlen 1))
+               (n ^- (natToWord addrlen 1))
+               l' nocrash crashed rx.
 Proof.
   intros.
-  unfold For_loop.
+  unfold For_.
   rewrite Fix_eq.
 
   destruct (weq n (natToWord addrlen 0)); f_equal.
@@ -202,7 +191,7 @@ Proof.
   apply functional_extensionality; auto.
 Qed.
 
-Theorem word_for_ok:
+Theorem for_ok':
   forall (n i : addr)
          (L : Set) (G : Type)
          f rx rec (nocrash : G -> addr -> L -> pred) (crashed : G -> pred)
@@ -215,7 +204,8 @@ Theorem word_for_ok:
       (forall lSm, {{ F * nocrash g (m ^+ (natToWord addrlen 1)) lSm }} (rxm lSm) >> rec) ->
       {{ F * nocrash g m lm }} f m lm rxm >> rec]]
    * [[forall lfinal, {{ F * nocrash g (n ^+ i) lfinal }} (rx lfinal) >> rec]]
-  }} (For_loop f i n li nocrash crashed rx) >> rec.
+   * [[wordToNat i + wordToNat n = wordToNat (i ^+ n)]]
+  }} (For_ f i n li nocrash crashed rx) >> rec.
 Proof.
   match goal with
   | [ |- forall (n: addr), ?P ] =>
@@ -229,15 +219,19 @@ Proof.
 
   - eapply pimpl_pre; repeat ( apply sep_star_lift_l; intros ).
     + unfold pimpl, lift; intros.
-      rewrite For_loop_step.
-      apply H1.
+      rewrite For_step.
+      apply H2.
     + fold (wzero addrlen). ring_simplify (wzero addrlen ^+ i). auto.
 
   - eapply pimpl_pre; repeat ( apply sep_star_lift_l; intros ).
-    + unfold pimpl, lift; intros.
-      rewrite For_loop_step.
+    + assert (wordToNat x <> 0).
+      unfold not in *; intros; apply n.
+      rewrite <- H5; rewrite natToWord_wordToNat; auto.
+
+      unfold pimpl, lift; intros.
+      rewrite For_step.
       rewrite H0.
-      apply H2.
+      apply H3.
 
       apply eq_le; auto.
       (* XXX i < x ^+ i: need something to prove non-overflow? *)
@@ -247,14 +241,27 @@ Proof.
       eapply pimpl_ok.
       apply H.
 
-      (* XXX [x ^- natToWord addrlen 1 < x] given [x <> natToWord addrlen 0] *)
-      admit.
+      apply lt_wlt.
+      rewrite wminus_Alt.
+      rewrite wminus_Alt2.
+      unfold wordBinN.
+      rewrite wordToNat_natToWord_idempotent'.
+      simpl; omega.
+      simpl (wordToNat (natToWord addrlen 1)).
+      eapply Nat.lt_le_trans; [| apply (wordToNat_bound x) ].
+      omega.
+      unfold not in *; intros; apply n.
+      apply wlt_lt in H7; simpl in H7.
+      rewrite <- natToWord_wordToNat with (w:=x).
+      f_equal.
+      omega.
+
       apply pimpl_exists_r; exists a.
       apply pimpl_exists_r; exists a0.
       repeat ( apply sep_star_lift_r; apply pimpl_and_split );
         unfold pimpl, lift; intuition eauto.
 
-      apply H2; eauto.
+      apply H3; eauto.
       (* XXX *)
       admit.
       (* XXX *)
@@ -262,51 +269,40 @@ Proof.
 
       ring_simplify (x ^- natToWord addrlen 1 ^+ (i ^+ natToWord addrlen 1)).
       eauto.
+
+      (* XXX *)
+      admit.
     + auto.
 Qed.
 
 Theorem for_ok:
-  forall (L : Set) (G : Type)
-         f rx rec (nocrash : G -> nat -> L -> pred) (crashed : G -> pred)
-         n i (li : L),
-  {{ exists F (g:G), F * nocrash g i li
+  forall (n : addr)
+         (L : Set) (G : Type)
+         f rx rec (nocrash : G -> addr -> L -> pred) (crashed : G -> pred)
+         (li : L),
+  {{ exists F (g:G), F * nocrash g (natToWord addrlen 0) li
    * [[forall m l, F * nocrash g m l ==> F * crashed g]]
    * [[forall m lm rxm,
-      i <= m < n + i ->
-      (forall lSm, {{ F * nocrash g (S m) lSm }} (rxm lSm) >> rec) ->
+      (m < n)%word ->
+      (forall lSm, {{ F * nocrash g (m ^+ (natToWord addrlen 1)) lSm }} (rxm lSm) >> rec) ->
       {{ F * nocrash g m lm }} f m lm rxm >> rec]]
-   * [[forall lfinal, {{ F * nocrash g (n+i) lfinal }} (rx lfinal) >> rec]]
-  }} (For_ f i n li nocrash crashed rx) >> rec.
+   * [[forall lfinal, {{ F * nocrash g n lfinal }} (rx lfinal) >> rec]]
+  }} (For_ f (natToWord addrlen 0) n li nocrash crashed rx) >> rec.
 Proof.
-  induction n.
-  - intros.
-    apply corr_exists; intros.
-    apply corr_exists; intros.
-    eapply pimpl_pre; repeat ( apply sep_star_lift_l; intros ).
-    + unfold pimpl; intuition pred.
-    + unfold pimpl; pred.
-  - intros.
-    apply corr_exists; intros.
-    apply corr_exists; intros.
-    eapply pimpl_pre; repeat ( apply sep_star_lift_l; intros ).
-    + unfold pimpl; intuition idtac.
-      eapply H0; try omega.
-      intros.
-      eapply pimpl_ok.
-      apply IHn.
-      apply pimpl_exists_r; exists a.
-      apply pimpl_exists_r; exists a0.
-      repeat ( apply sep_star_lift_r; apply pimpl_and_split );
-        unfold pimpl, lift; intuition eauto.
-      apply H0; eauto; omega.
-      replace (n + S i) with (S (n + i)) by omega; eauto.
-    + unfold pimpl; pred.
+  intros.
+  eapply pimpl_ok.
+  apply for_ok'.
+  fold (wzero addrlen); ring_simplify (wzero addrlen ^+ n).
+  simpl (wordToNat (wzero addrlen)); replace (0 + wordToNat n) with (wordToNat n) by omega.
+  ring_simplify (n ^+ wzero addrlen).
+  cancel.
+  cancel.
 Qed.
 
 Hint Extern 1 ({{_}} progseq (For_ _ _ _ _ _ _) _ >> _) => apply for_ok : prog.
 Notation "'For' i < n 'Loopvar' l <- l0 'Continuation' lrx 'Invariant' nocrash 'OnCrash' crashed 'Begin' body 'Rof'" :=
   (For_ (fun i l lrx => body)
-        0 n l0
+        (natToWord addrlen 0) n l0
         (fun (_:unit) i l => nocrash%pred)
         (fun (_:unit) => crashed%pred))
   (at level 9, i at level 0, n at level 0, lrx at level 0, l at level 0, l0 at level 0,
@@ -314,7 +310,7 @@ Notation "'For' i < n 'Loopvar' l <- l0 'Continuation' lrx 'Invariant' nocrash '
 
 Notation "'For' i < n 'Ghost' g1 .. g2 'Loopvar' l <- l0 'Continuation' lrx 'Invariant' nocrash 'OnCrash' crashed 'Begin' body 'Rof'" :=
   (For_ (fun i l lrx => body)
-        0 n l0
+        (natToWord addrlen 0) n l0
         (pair_args_helper (fun g1 => .. (pair_args_helper (fun g2 (_:unit) =>
          fun i l => nocrash%pred)) .. ))
         (pair_args_helper (fun g1 => .. (pair_args_helper (fun g2 (_:unit) =>
